---
layout: post
title: Assignment 2
author: Kapil Chaudhary
---
## Solution 1

Given differential equation is :

$$x(1-x^2)dy + (2x^2 y -y-a x^3)dx=0 $$

Comparing with $M dx + N dy =0$ , We have
$  M=(2x^2 y -y-a x^3) $ and $ N = x(1-x^2) $

$$ \frac{\delta M}{\delta y} = \frac{\delta }{\delta y}(2x^2 y -y-a x^3) \\ = 2x^2 -1$$

$$ \frac{\delta N}{\delta x} = \frac{\delta }{\delta x}  x(1-x^2) \\ = 1-3x^2 $$

$$ \frac{\delta M}{\delta y} -\frac{\delta N}{\delta x} =  2x^2-1-1+3x^2 \\ 5x^2-2 $$
